\section{Формула Тейлора для многочленов}

\begin{lemma}

    Пусть $f(x) = (x -x_0)^k$, тогда $f^{(m)}(x_0) =
    \begin{cases}
        m! &\text{if $k=m$}\\
        0 &\text{else}
    \end{cases}$
\end{lemma}
\begin{proof}
    \begin{itemize}
        \item $k \geq m$, тогда $f^{(m)}(x) = k(k-1) \dots (k-m+1)(x-x_0)^{k-m}$:
        \begin{itemize}
            \item $k = m$, тогда $f^{(m)}(x) = k! = m!$
            \item $k > m$, тогда $f^{(m)}(x) = c (x-x_0)^{k-m} \Longrightarrow f^{(m)}(x_0) = 0$
        \end{itemize}
        
        \item $k < m$, тогда $(f^{(k)})^{(m-k)} = (k!)^{(m-k)} = 0$
    \end{itemize}
\end{proof}
\
\begin{theorem-non}
    Формула Тейлора для многочлена

    $T$ --- многочлен, $deg T = n$. тогда

    $T(x) = \sum\limits_{k=0}^n \frac{T^{(k)}(x_0)}{k!} (x-x_0)^k$
\end{theorem-non}
\begin{proof}
    $T(x) = \sum\limits_{k = 0}^{n} c_k (x-x_0)^k$ \quad надо доказать, что $c_k = \frac{T^{(n)}(x_0)}{k!}$

    $T^{(m)}(x_0) = \left.\sum\limits_{k = 0}^{n} c_k ((x-x_0)^k)^{(m)} \right|_{x=x_0} = c_m \cdot m!$ (по лемме)

    Тогда $c_m = \frac{T^{(m)}(x_0)}{m!}$
\end{proof}

